chore: add fsmEqUpto for unary
This shows what it means to check for unary equality.

SSA/Experimental/Bits/MultiWidth/GoodFSM.lean
@@ -88,7 +88,6 @@ def IsGoodNatFSM_mkWidthFSM {wcard : Nat} (tcard : Nat) {w : WidthExpr wcard} :
 def fsmUleUnary (a : FSM α) (b : FSM α) : FSM α :=
  composeUnaryAux FSM.scanAnd (b ||| ~~~ a)
 
-@[simp]
 theorem eval_fsmUltUnary_eq_decide
     (a : NatFSM wcard tcard (.ofDep v))
     (b : NatFSM wcard tcard (.ofDep w))
@@ -140,14 +139,77 @@ theorem eval_fsmUltUnary_eq_decide
             exists (wenv v)
             omega
 
+@[simp]
+theorem eval_fsmUltUnary_eq_lt_or_decide
+    (a : NatFSM wcard tcard (.ofDep v))
+    (b : NatFSM wcard tcard (.ofDep w))
+    {wenv : WidthExpr.Env wcard}
+    {fsmEnv : StateSpace wcard tcard → BitStream}
+    (henv : HWidthEnv fsmEnv wenv)
+    (ha : IsGoodNatFSM a) (hb : IsGoodNatFSM b) :
+    ((fsmUleUnary a.toFsm b.toFsm).eval fsmEnv) i =
+    decide (i ≤ min (v.toNat wenv) (w.toNat wenv) ∨ (v.toNat wenv) ≤ (w.toNat wenv)) := by
+  rw [eval_fsmUltUnary_eq_decide (wenv := wenv) (henv := henv) (ha := ha) (hb := hb)]
+  simp
+  by_cases hiv : i ≤ v.toNat wenv
+  · simp [hiv]
+  · simp [hiv]
+    omega
 /--
 info: 'MultiWidth.eval_fsmUltUnary_eq_decide' depends on axioms: [propext, Classical.choice, Quot.sound]
 -/
 #guard_msgs in #print axioms eval_fsmUltUnary_eq_decide
 
 -- returns 1 if a is equal to b.
-def fsmEqUpto (a : FSM α) (b : FSM α) : FSM α :=
-  composeUnaryAux FSM.scanAnd <| composeBinaryAux' FSM.nxor a  b
+def fsmEqUnaryUpto (a : FSM α) (b : FSM α) : FSM α :=
+  composeUnaryAux FSM.scanAnd (composeBinaryAux' FSM.nxor a b)
+
+
+@[simp]
+private theorem min_eq_of_not_le {a b : Nat} (hab : ¬ a ≤ b) : min a b = b := by
+  omega
+
+@[simp]
+private theorem min_eq_of_not_le' {a b : Nat} (hab : ¬ a ≤ b) : min b a = b := by
+  omega
+
+
+theorem eval_FsmEqUpto_eq_decide
+    (a : NatFSM wcard tcard (.ofDep v))
+    (b : NatFSM wcard tcard (.ofDep w))
+    {wenv : WidthExpr.Env wcard}
+    {fsmEnv : StateSpace wcard tcard → BitStream}
+    (henv : HWidthEnv fsmEnv wenv)
+    (ha : IsGoodNatFSM a) (hb : IsGoodNatFSM b) :
+    ((fsmEqUnaryUpto a.toFsm b.toFsm).eval fsmEnv) i =
+    decide (min i (v.toNat wenv) = min i (w.toNat wenv)) := by
+  simp [fsmEqUnaryUpto]
+  rw [ha.heq (henv := henv)]
+  rw [hb.heq (henv := henv)]
+  induction w generalizing v
+  case var w =>
+    induction v
+    case var v =>
+      simp [BitStream.scanAnd_eq_decide]
+      constructor
+      · intros hi
+        -- | think about what the heck this is saying.
+        by_cases hiv : wenv v ≤ i
+        · have hiv' := hi (wenv v) hiv
+          have := hiv'.mp (by simp)
+          simp [hiv]
+          by_cases hiw : wenv w ≤ i
+          · simp [hiw]
+            have hiw' := hi (wenv w) hiw
+            have := hiw'.mpr (by simp)
+            omega
+          · simp [hiw]
+            have hiv' := hi i (by simp) |>.mpr (by omega)
+            omega
+        · simp [hiv]
+          apply hi .. |>.mp <;> omega
+      · intros hivw j hj
+        omega
 
 
 -- | if 'cond' is true, then return 't', otherwise return 'e'.
@@ -264,7 +326,7 @@ def mkPredicateFSMAux (wcard tcard : Nat) (p : Nondep.Predicate) :
   | .binRel .eq a b =>
     let fsmA := mkTermFSM wcard tcard a
     let fsmB := mkTermFSM wcard tcard b
-    { toFsm := fsmEqUpto fsmA.toFsm fsmB.toFsm }
+    { toFsm := fsmEqUnaryUpto fsmA.toFsm fsmB.toFsm }
   | .or p q  =>
     let fsmP :=  mkPredicateFSMAux wcard tcard p
     let fsmQ :=  mkPredicateFSMAux wcard tcard q
